cfrontend/PrintCsyntax.ml
@@ -18,7 +18,6 @@
 
 open Format
 open Camlcoq
-open Values
 open AST
 open! Ctypes
 open Tags
@@ -31,9 +30,11 @@ module PrintCsyntaxP =
 
 module C2CPInst = C2CP (Pol) (Alloc)
 module Init = C2CPInst.Init
-module Ctyping = Init.Cexec.InterpreterEvents.Ctyping
+module Ctyping = Init.Cexec.InterpreterEvents.Deterministic.Ctyping
 module Csyntax = Ctyping.Csem.Csyntax
 module Cop = Csyntax.Cop
+module Val = Ctyping.Outer.M.MD.TLib.Switch.BI.BI1.BI0.Values
+open Val
 
 let name_unop = function
   | Values.Onotbool -> "!"
@@ -199,6 +200,8 @@ let print_typed_value p vty =
   | (Vlong n, Ctypes.Tlong(Unsigned, _)) ->
       fprintf p "%LuLLU" (camlint64_of_coqint n)
   | (Vlong n, _) ->
+      fprintf p "%LdLL" (camlint64_of_coqint n)
+  | (Vptr n, _) ->
       fprintf p "%LdLL" (camlint64_of_coqint n)
   | (Vfptr b, _) ->
       fprintf p "<ptr%a>" !print_pointer_hook (b,coqint_of_camlint 0l)
