common/Globalenvs.v
@@ -204,8 +204,8 @@ Module Genv (Ptr: Pointer) (Pol: Policy) (M:Memory Ptr Pol) (A: Allocator Ptr Po
         let diff := Nat.sub n (length idl) in
         idl ++ (repeat (Init_int8 Int.zero) diff).
             
-      Definition alloc_global (ge: t) (m: mem) (c: context)
-                 (tree: PTree.t (context -> ptr)) (id: ident) (v: globvar V)
+      Definition alloc_global (ge: t) (m: mem)
+                 (tree: PTree.t ptr) (id: ident) (v: globvar V)
                  (vt : val_tag) (lt : loc_tag) : PolicyResult (ptr * mem) :=
         let init := v.(gvar_init) in
         let sz := v.(gvar_size) in
@@ -213,18 +213,18 @@ Module Genv (Ptr: Pointer) (Pol: Policy) (M:Memory Ptr Pol) (A: Allocator Ptr Po
         match PTree.get id tree with
         | Some base =>
             let padded := pad_init_data_list (Pos.to_nat sz) init in
-            m2 <- store_init_data_list ge m (base c) padded vt lt;;
-            ret (base c,m2)
+            m2 <- store_init_data_list ge m base padded vt lt;;
+            ret (base,m2)
         | None => raise (OtherFailure "Globals weren't allocated correctly")
         end.
 
-      Program Definition add_global (ge: t) (m: mem) (c: context)
-              (tree: PTree.t (context -> ptr)) (idg: ident * globdef F V)
+      Program Definition add_global (ge: t) (m: mem)
+              (tree: PTree.t ptr) (idg: ident * globdef F V)
         : PolicyResult (t*mem) :=
         match idg#2 with
         | Gvar gv =>
             let '(pt, vt, lt) := GlobalT ce (idg#1) Tvoid in (* TODO: if we're going to do things based on type here, need to concretize V *)
-            '(base', m') <- alloc_global ge m c tree (idg#1) gv vt lt;;
+            '(base', m') <- alloc_global ge m tree (idg#1) gv vt lt;;
             let size := Int64.repr (Zpos gv.(gvar_size)) in
             let bound := off base' size in
             let genv_symb' := PTree.set idg#1 (SymGlob base' bound pt gv) ge.(genv_symb) in
@@ -311,14 +311,14 @@ Module Genv (Ptr: Pointer) (Pol: Policy) (M:Memory Ptr Pol) (A: Allocator Ptr Po
         - eapply ge.(genv_funs_inj); eauto.        
       Defined.
       
-      Fixpoint add_globals (ge: t) (cs: ident -> context) (m: mem)
-               (tree: PTree.t (context -> ptr)) (gl: list (ident * globdef F V))
+      Fixpoint add_globals (ge: t) (m: mem)
+               (tree: PTree.t ptr) (gl: list (ident * globdef F V))
         : PolicyResult (t*mem) :=
         match gl with
         | [] => ret (ge,m)
         | g::gl' =>
-           '(ge', m') <- add_globals ge cs m tree gl';;
-            add_global ge' m' (cs (fst g)) tree g
+           '(ge', m') <- add_globals ge m tree gl';;
+            add_global ge' m' tree g
         end.
       
       Program Definition empty_genv (pub: list ident) : t :=
@@ -331,10 +331,10 @@ Module Genv (Ptr: Pointer) (Pol: Policy) (M:Memory Ptr Pol) (A: Allocator Ptr Po
         | _::idgs' => filter_var_sizes idgs'
         end.
       
-      Definition globalenv (p: AST.program F V) (cs: ident -> context) :
+      Definition globalenv (p: AST.program F V) :
         PolicyResult (t * mem) :=
         let (m,tree) := A.globalalloc A.empty (filter_var_sizes p.(AST.prog_defs)) in
-        (add_globals (empty_genv p.(AST.prog_public)) cs m tree p.(AST.prog_defs)).
+        (add_globals (empty_genv p.(AST.prog_public)) m tree p.(AST.prog_defs)).
       Section WITH_GE.
 
         Variable ge : t.
